DumbContracts/Proofs/Counter/Basic.lean
@@ -164,7 +164,7 @@ theorem increment_twice_adds_two (s : ContractState) :
       = EVM.Uint256.add (((increment).run s).snd.storage 0) 1 := h2
     _ = EVM.Uint256.add (EVM.Uint256.add (s.storage 0) 1) 1 := by rw [h1]
 
-theorem increment_decrement_cancel (s : ContractState) (h_range : s.storage 0 < 2^256) :
+theorem increment_decrement_cancel (s : ContractState) :
   let s' := ((increment).run s).snd
   let s'' := ((decrement).run s').snd
   s''.storage 0 = s.storage 0 := by
@@ -176,9 +176,7 @@ theorem increment_decrement_cancel (s : ContractState) (h_range : s.storage 0 < 
       = EVM.Uint256.sub (((increment).run s).snd.storage 0) 1 := h2
     _ = EVM.Uint256.sub (EVM.Uint256.add (s.storage 0) 1) 1 := by rw [h1]
     _ = s.storage 0 := by
-      have h_one : (1:Nat) < 2^256 := by
-        simp_arith
-      simpa using (EVM.Uint256.sub_add_cancel_of_lt h_range h_one)
+      simpa using (EVM.Uint256.sub_add_cancel (s.storage 0) 1)
 
 /-! ## State Preservation -/
 
